examples/Auto/Demo.v
@@ -1,0 +1,256 @@
+Require Import ExtLib.Core.RelDec.
+Require Import ExtLib.Tactics.
+Require Import MirrorCore.SymI.
+Require Import MirrorCore.EProverI.
+Require Import MirrorCore.Lemma.
+Require Import MirrorCore.Lambda.Expr.
+Require Import MirrorCore.syms.SymEnv.
+Require Import MirrorCore.provers.AssumptionProver.
+Require Import MirrorCore.Subst.FMapSubst.
+Require Import MirrorCore.provers.AutoProver.
+Require Import McExamples.Simple.Simple.
+
+Set Implicit Arguments.
+Set Strict Implicit.
+
+Inductive Even : nat -> Prop :=
+| Even_0 : Even 0
+| Even_SS : forall n, Even n -> Even (S (S n)).
+
+Theorem Even_plus : forall n m,
+                      Even n -> Even m ->
+                      Even (n + m).
+Proof.
+  induction 1; simpl; intros; auto.
+  apply Even_SS. auto.
+Qed.
+
+Theorem Even_minus : forall n m,
+                       Even n -> Even m ->
+                       Even (n - m).
+Proof.
+  intros n m H. revert m.
+  induction H; simpl; intros; auto.
+  { constructor. }
+  { destruct H0.
+    { constructor. specialize (IHEven 0 Even_0).
+      rewrite <- Minus.minus_n_O in IHEven. auto. }
+    { eauto. } }
+Qed.
+
+Definition fs : @functions typ _ :=
+  Eval simpl in from_list
+                  ((@F typ _ (tyArr tyNat tyProp) (fun _ => Even)) ::
+                   (@F typ _ tyNat (fun _ => O)) ::
+                   (@F typ _  (tyArr tyNat tyNat) (fun _ => S)) ::
+                   (@F typ _  (tyArr tyNat (tyArr tyNat tyNat)) (fun _ => plus)) ::
+                   (@F typ _  (tyArr tyNat (tyArr tyNat tyNat)) (fun _ => minus)) ::
+                   nil).
+
+Let func := SymEnv.func.
+
+Fixpoint makeNat (n : nat) : expr typ func :=
+  match n with
+    | O => Inj (2)
+    | S n => App (Inj 3) (makeNat n)
+  end%positive.
+
+Let RSym_func : @RSym typ _ func := SymEnv.RSym_func fs.
+Local Existing Instance RSym_func.
+
+Let Expr_expr : @ExprI.Expr typ _ (expr typ func) := Expr_expr.
+Local Existing Instance Expr_expr.
+
+Definition lem_0 : lemma typ (expr typ func) (expr typ func) :=
+  Eval simpl makeNat in
+    {| vars := nil ; premises := nil ; concl := App (Inj 1%positive) (makeNat 0) |}.
+
+Definition lem_SS : lemma typ (expr typ func) (expr typ func) :=
+  {| vars := tyNat :: nil
+     ; premises := App (Inj 1%positive) (Var 0) :: nil
+     ; concl := App (Inj 1%positive)
+                    (App (Inj 3%positive) (App (Inj 3%positive) (Var 0)))
+  |}.
+
+Definition lem_plus : lemma typ (expr typ func) (expr typ func) :=
+  {| vars := tyNat :: tyNat :: nil
+   ; premises := App (Inj 1%positive) (Var 0) ::
+                 App (Inj 1%positive) (Var 1) :: nil
+   ; concl := App (Inj 1%positive)
+                  (App (App (Inj 4%positive) (Var 0)) (Var 1))
+  |}.
+
+Definition lem_minus : lemma typ (expr typ func) (expr typ func) :=
+  {| vars := tyNat :: tyNat :: nil
+   ; premises := App (Inj 1%positive) (Var 0) ::
+                 App (Inj 1%positive) (Var 1) :: nil
+   ; concl := App (Inj 1%positive)
+                  (App (App (Inj 5%positive) (Var 0)) (Var 1))
+  |}.
+
+
+Definition evenHints : Hints typ (expr typ func) :=
+{| Apply := lem_0 :: lem_SS :: lem_plus :: lem_minus :: nil
+ ; Extern := from_Prover (@assumptionProver _ (expr typ func) _)
+ |}.
+
+Instance ExprOk_expr : ExprI.ExprOk Expr_expr := @ExprOk_expr _ _ _ _ _ _ _ _ nil.
+
+Theorem evenHintsOk : @HintsOk _ _ RType_typ _ _ evenHints.
+Proof.
+  constructor.
+  { unfold evenHints; simpl.
+    repeat (apply Forall_cons || apply Forall_nil).
+    exact Even_0.
+    exact Even_SS.
+    exact Even_plus.
+    exact Even_minus. }
+  { unfold evenHints; simpl.
+    eapply from_ProverT_correct; eauto with typeclass_instances.
+    apply (@assumptionProver_correct typ _ (expr typ func) _ _ _ _ _). }
+Qed.
+
+
+
+Let subst := FMapSubst.SUBST.raw (expr typ func).
+Local Instance Subst_subst : SubstI.Subst subst (expr typ func) := FMapSubst.SUBST.Subst_subst _.
+Local Instance SubstUpdate_subst : SubstI.SubstUpdate subst (expr typ func) := FMapSubst.SUBST.SubstUpdate_subst _.
+eapply instantiate.
+Defined.
+
+Local Instance SubstOk_fmap_subst : @SubstI.SubstOk _ _ _ _ _ Subst_subst :=
+  @FMapSubst.SUBST.SubstOk_subst _ _ _ _ _.
+Local Instance SubstUpdateOk_fmap_subst : @SubstI.SubstUpdateOk subst typ _ (expr typ func) _ _ (SubstUpdate_subst) _.
+eapply (@FMapSubst.SUBST.SubstUpdateOk_subst _ _ _ _ _).
+eapply ExprSubst.instantiate_mentionsU.
+eapply ExprSubst.exprD'_instantiate; eauto with typeclass_instances.
+Qed.
+
+Require MirrorCore.Lambda.ExprUnify_simul.
+
+Theorem Apply_auto_prove (fuel : nat) hints (Hok : HintsOk _ _ hints)
+: forall facts (us vs : EnvI.env nil) goal s',
+    @auto_prove typ (expr typ func) _ _ subst _ _ 
+                hints
+                (vars_to_uvars)
+                (fun tus tvs under el er (t : typ) (sub : subst) =>
+                   @ExprUnify_simul.exprUnify _ _ _ _ _ _ _ _ 10 nil tus tvs under sub el er t)
+                (@instantiate typ func) fuel facts
+                (EnvI.typeof_env us) (EnvI.typeof_env vs) goal
+                (@SubstI.empty _ _ _) = Some s' ->
+    (let (tus,us) := EnvI.split_env us in
+     let (tvs,vs) := EnvI.split_env vs in
+     match @SubstI.substD _ _ _ _ _ _ _ tus tvs s' with
+       | None => False
+       | Some P => P us vs
+     end) ->
+    match @ExprI.exprD _ RType_typ _ _ us vs goal tyProp return Prop with
+      | None => True
+      | Some P => P
+    end.
+Proof.
+Admitted.
+
+Goal Even 0.
+Proof.
+  pose (goal := App (Inj 1%positive) (makeNat 0)).
+  change match ExprI.exprD (Expr := Expr_expr) nil nil goal tyProp with
+           | None => True
+           | Some P => P
+         end.
+  eapply (@Apply_auto_prove 100 evenHints evenHintsOk
+                            (evenHints.(Extern).(Summarize) nil nil nil)).
+  compute. reflexivity.
+  compute. auto.
+Qed.
+
+(*
+Goal Even 2.
+Proof.
+  pose (goal := App (Inj 1%positive) (makeNat 2)).
+  change match exprD nil nil goal tyProp with
+           | None => True
+           | Some P => P
+         end.
+  eapply (@Apply_auto_prove 100 evenHints evenHintsOk
+                            (evenHints.(Extern).(Summarize) nil nil nil)).
+  compute. reflexivity.
+  compute. auto.
+Qed.
+*)
+
+Goal Even 200.
+Proof.
+  pose (goal := App (Inj 1%positive) (makeNat 200)).
+  change match ExprI.exprD (Expr := Expr_expr) nil nil goal tyProp with
+           | None => True
+           | Some P => P
+         end.
+  eapply (@Apply_auto_prove 101 evenHints evenHintsOk
+                            (evenHints.(Extern).(Summarize) nil nil nil)).
+  match goal with
+    | |- ?X = Some ?Y =>
+      let res := eval vm_compute in X in
+                                     (etransitivity ; [ | exact (@eq_refl _ res) ])
+  end.
+  Time vm_compute; reflexivity.
+  compute. reflexivity.
+Qed.
+(** vm_compute is still *very* slow for this!
+ ** - Some optimizations might be possible
+ **   - Make unification faster, e.g. special-case fully instantiated terms
+ **     so you don't keep instantiating them.
+ **   - eliminate fully instantiated unification variables
+ **)
+
+Goal Even 200.
+Proof.
+  Time eauto 200 using Even_0, Even_SS.
+Qed.
+
+Goal Even ((200 + 200) + 200).
+Proof.
+  Time eauto 400 using Even_0, Even_SS, Even_plus.
+Qed.
+
+Definition seven : expr typ func -> expr typ func := 
+  App (Inj 1%positive).
+Definition splus (l r : expr typ func) : expr typ func := App (App (Inj 4%positive) l) r.
+
+Goal Even (0 + 0).
+Proof.
+  pose (goal := seven (splus (makeNat 0) (makeNat 0))).
+  (** This is problematic because it is going to actually compute 600? **)
+  Time change match ExprI.exprD (Expr := Expr_expr) nil nil goal tyProp with
+                | None => True
+                | Some P => P
+              end.
+  eapply (@Apply_auto_prove 2 evenHints evenHintsOk
+                            (evenHints.(Extern).(Summarize) nil nil nil)).
+  match goal with
+    | |- ?X = Some ?Y =>
+      let res := eval vm_compute in X in
+      (etransitivity ; [ | exact (@eq_refl _ res) ])
+  end.
+  Time (vm_compute; reflexivity).
+  compute. trivial.
+Qed.
+
+Goal Even ((200 + 200) + 200).
+Proof.
+  pose (goal := seven (splus (splus (makeNat 200) (makeNat 200)) (makeNat 200))).
+  (** This is problematic because it is going to actually compute 600? **)
+  Time change match ExprI.exprD (Expr := Expr_expr) nil nil goal tyProp with
+                | None => True
+                | Some P => P
+              end.
+  eapply (@Apply_auto_prove 203 evenHints evenHintsOk
+                            (evenHints.(Extern).(Summarize) nil nil nil)).
+  match goal with
+    | |- ?X = Some ?Y =>
+      let res := eval vm_compute in X in
+      (etransitivity ; [ | exact (@eq_refl _ res) ])
+  end.
+  Time vm_compute; reflexivity.
+  compute. trivial.
+Qed.
