theories/Lambda/Expr.v
@@ -1,2 +1,4 @@
 Require Export MirrorCore.Lambda.ExprCore.
 Require Export MirrorCore.Lambda.ExprD.
+Require Export MirrorCore.Lambda.ExprLift.
+Require Export MirrorCore.Lambda.ExprSubst.
