theories/Lambda/ExprLift.v
@@ -7,7 +7,8 @@ Require Import ExtLib.Tactics.
 Require Import MirrorCore.SymI.
 Require Import MirrorCore.EnvI.
 Require Import MirrorCore.TypesI.
-Require Import MirrorCore.Lambda.Expr.
+Require Import MirrorCore.Lambda.ExprCore.
+Require Import MirrorCore.Lambda.ExprD.
 
 Set Implicit Arguments.
 Set Strict Implicit.
